Created: Aug 27 2025
Class: [[Maths]] 
- - -
$$
For: p\rightarrow c
$$
$$
Prove: \neg c \rightarrow \neg p
$$
## Multiple hypothesis
For 
$$
H_1 \wedge H_2 \rightarrow C
$$
Contrapositive:
$$
\neg C \rightarrow \neg(H_1 \land H_2)
$$
$$
\neg C \rightarrow (\neg H_1 \lor \neg H_2)
$$
                                     ^^^^^^^^^^^ Commutative law can be used to reorder hypothesises
$$
C \space \lor \neg H_1 \lor \neg H_2
$$
$$
(C \space \lor  \neg H_1) \lor \neg H_2
$$
$$
(\neg C \land H_1) \rightarrow \neg H_2
$$
